impossibilite/package-disc13/MeetingTheorem_FAIR.v
@@ -1,6 +1,6 @@
 Set Implicit Arguments.
-Require Import ConvergentFormalism3.
-(* Require Import FiniteSum. *)
+Require Import ConvergentFormalism.
+Require Import FiniteSum.
 Require Import Field.
 Require Import Qcanon.
 Require Import Qcabs.
@@ -35,22 +35,6 @@ Proof.
   + eleft; simpl; unfold inv; split.
 Qed.
 
-Lemma demon1_is_fully_synchronous: forall q d g b, FullySynchronous (demon1 d g b q).
-Proof.
-  cofix.
-  intros q.
-  constructor.  
-  - unfold demon1.
-    intros g'.
-    constructor.
-    simpl.
-    discriminate.
-  - simpl. 
-    fold (demon1 d g b).
-    apply demon1_is_fully_synchronous.
-Qed.    
-
-
 Lemma S1 g b (x : name g) (r : robogram g b) (l : Qc)
 : forall (gp : name g -> Qc) (k : Qc), (forall g, gp g = k) ->
   imprisonned l [delta r] (execute r (demon1 (delta r) g b (1 + k)) gp) ->
@@ -73,7 +57,7 @@ Proof.
         unfold round; simpl; unfold similarity; simpl; intros; rewrite Hgp.
         rewrite (@AlgoMorph g b r _ (pos0 g b) (id_perm g b));
         [fold (delta r); field; discriminate|].
-        split; simpl; intros; [rewrite Hgp|]; ring.
+        split;simpl; intros; [rewrite Hgp|] ; ring.
       * destruct Himp.
         revert Himp; clear.
         simpl; fold (demon1 (delta r) g b) (execute r).
@@ -141,54 +125,11 @@ Proof.
         now rewrite Qcplus_assoc.
 Qed.
 
-Lemma S2' g b (x : name g) (r : robogram g b) : solution_FSYNC r -> ~ 0 < [delta r].
-Proof.
-  intros Hs H.
-  destruct (Hs (fun _=>0) (demon1 (delta r) g b 1) (demon1_is_fully_synchronous _ _ _ _)
-               [delta r] H) as [lim Hlim].
-  cut (forall (gp : name g -> Qc) (k : Qc), (forall g, gp g = k) ->
-       attracted lim [delta r] (execute r (demon1 (delta r) g b (1 + k)) gp) ->
-       [delta r] = 0).
-  + intros K.
-    generalize (K (fun _ => 0) 0 (fun x => eq_refl 0)); clear K.
-    rewrite Qcplus_0_r; intros K; rewrite (K Hlim) in H; clear - H.
-    discriminate.
-  + clear - x.
-    intros.
-    remember (execute r (demon1 (delta r) g b (1+k)) gp).
-    revert gp k H Heqe.
-    induction H0; intros; subst.
-    - eapply S1; eauto.
-    - clear H0.
-      apply (IHattracted (round r {|byz_replace:=fun _=>1+k
-                                       ;frame:=fun _=>1|} gp)
-                         (k + delta r)).
-      * clear - H.
-        intros g0; unfold round; simpl; unfold similarity; simpl.
-        rewrite (@AlgoMorph g b r _ (pos0 g b) (id_perm g b));
-        [fold (delta r); rewrite H; field; discriminate|].
-        split; intros; simpl; repeat rewrite H; ring_simplify; split.
-      * simpl; clear.
-        fold (demon1 (delta r) g b) (execute r).
-        now rewrite Qcplus_assoc.
-Qed.
-
 Theorem meeting_theorem g b (x : name g) (r : robogram g b)
 : solution r -> delta r = 0.
 Proof.
   intros Hs.
   generalize (S2 x Hs); generalize (delta r); clear.
-  intros q Hneg.
-  generalize (proj1 (Qcabs_Qcle_condition _ _) (Qcnot_lt_le _ _ Hneg)); clear.
-  intros [A B]; apply Qcle_antisym; auto.
-Qed.
-
-
-Theorem meeting_theorem' g b (x : name g) (r : robogram g b)
-: solution_FSYNC r -> delta r = 0.
-Proof.
-  intros Hs.
-  generalize (S2' x Hs); generalize (delta r); clear.
   intros q Hneg.
   generalize (proj1 (Qcabs_Qcle_condition _ _) (Qcnot_lt_le _ _ Hneg)); clear.
   intros [A B]; apply Qcle_antisym; auto.
